abp/SenderAutomaton.thy
@@ -3,22 +3,13 @@
  * This file was generated from Sender.maa and will be overridden when changed. To change
  * permanently, consider changing the model itself.
  *
- * Generated on Oct 1, 2018 2:45:43 PM by isartransformer 1.0.0
+ * isartransformer 1.0.0
  *)
 theory SenderAutomaton
   imports bundle.tsynBundle automat.dAutomaton
 
 begin
 
-
-(* TODO Sollte wahrscheinlich in OptionCpo sein? *)
-lemma option_one_cont: "cont (\<lambda>x. [c \<mapsto> f\<cdot>x])"
-  apply(rule contI2, rule monofunI)
-  apply (simp add: below_option_def fun_belowI monofun_cfun_arg)
-  apply (auto simp add: below_fun_def below_option_def)
-  apply (smt below_option_def chain_monofun domIff fun_belowI fun_upd_apply option.exhaust_sel part_dom_lub po_class.chain_def some_below)
-  apply (simp add: contlub_cfun_arg part_map_chain part_the_lub)
-  by (smt below_option_def cont_pref_eq1I domIff fun_belowI fun_upd_apply option.sel option.simps(3) part_dom_lub po_class.chain_def)
 
 (* Helper for easier generation *)
 fun prepend :: "'a::type list \<Rightarrow> 'a \<Rightarrow> 'a list" where
@@ -27,7 +18,7 @@ fun prepend :: "'a::type list \<Rightarrow> 'a \<Rightarrow> 'a list" where
 
 section \<open>Datatype definition\<close>
 
-datatype ('e::countable) senderMessage = DoNotUse_68fffe8e525945708a2c302dfe2fe6ec_SenderBool "bool" | DoNotUse_68fffe8e525945708a2c302dfe2fe6ec_SenderE "'e" | DoNotUse_68fffe8e525945708a2c302dfe2fe6ec_SenderPair_E_Bool "('e\<times>bool)"
+datatype ('e::countable) senderMessage = DoNotUse_d60d54060b9d448ea60e06d4478b7275_SenderBool "bool" | DoNotUse_d60d54060b9d448ea60e06d4478b7275_SenderE "'e" | DoNotUse_d60d54060b9d448ea60e06d4478b7275_SenderPair_E_Bool "('e\<times>bool)"
 
 instance senderMessage :: (countable) countable
   apply(intro_classes)
@@ -37,9 +28,9 @@ instantiation senderMessage :: (countable) message
 begin
   fun ctype_senderMessage :: "channel \<Rightarrow> ('e::countable) senderMessage set" where
   "ctype_senderMessage c = (
-    if c = \<C> ''DoNotUse_68fffe8e525945708a2c302dfe2fe6ec_as'' then range DoNotUse_68fffe8e525945708a2c302dfe2fe6ec_SenderBool else
-    if c = \<C> ''DoNotUse_68fffe8e525945708a2c302dfe2fe6ec_i'' then range DoNotUse_68fffe8e525945708a2c302dfe2fe6ec_SenderE else
-    if c = \<C> ''DoNotUse_68fffe8e525945708a2c302dfe2fe6ec_ds'' then range DoNotUse_68fffe8e525945708a2c302dfe2fe6ec_SenderPair_E_Bool else
+    if c = \<C> ''DoNotUse_d60d54060b9d448ea60e06d4478b7275_as'' then range DoNotUse_d60d54060b9d448ea60e06d4478b7275_SenderBool else
+    if c = \<C> ''DoNotUse_d60d54060b9d448ea60e06d4478b7275_i'' then range DoNotUse_d60d54060b9d448ea60e06d4478b7275_SenderE else
+    if c = \<C> ''DoNotUse_d60d54060b9d448ea60e06d4478b7275_ds'' then range DoNotUse_d60d54060b9d448ea60e06d4478b7275_SenderPair_E_Bool else
     undefined)"
   instance
     by(intro_classes)
@@ -49,30 +40,30 @@ end
 section \<open>Domain and range\<close>
 
 definition senderDom :: "channel set" where
-"senderDom = {\<C> ''DoNotUse_68fffe8e525945708a2c302dfe2fe6ec_as'', \<C> ''DoNotUse_68fffe8e525945708a2c302dfe2fe6ec_i''}"
+"senderDom = {\<C> ''DoNotUse_d60d54060b9d448ea60e06d4478b7275_as'', \<C> ''DoNotUse_d60d54060b9d448ea60e06d4478b7275_i''}"
 
 definition senderRan :: "channel set" where
-"senderRan = {\<C> ''DoNotUse_68fffe8e525945708a2c302dfe2fe6ec_ds''}"
+"senderRan = {\<C> ''DoNotUse_d60d54060b9d448ea60e06d4478b7275_ds''}"
 
 
 section \<open>Helpers to create a bundle from a single raw element\<close>
 
 lift_definition senderElem_raw_as :: "bool \<Rightarrow> ('e::countable) senderMessage tsyn sbElem" is
-"\<lambda>x. [\<C> ''DoNotUse_68fffe8e525945708a2c302dfe2fe6ec_as'' \<mapsto> Msg (DoNotUse_68fffe8e525945708a2c302dfe2fe6ec_SenderBool x)]"
+"\<lambda>x. [\<C> ''DoNotUse_d60d54060b9d448ea60e06d4478b7275_as'' \<mapsto> Msg (DoNotUse_d60d54060b9d448ea60e06d4478b7275_SenderBool x)]"
   unfolding sbElemWell_def
   unfolding usclOkay_stream_def
   unfolding ctype_tsyn_def
   by simp
 
 lift_definition senderElem_raw_i :: "'e \<Rightarrow> ('e::countable) senderMessage tsyn sbElem" is
-"\<lambda>x. [\<C> ''DoNotUse_68fffe8e525945708a2c302dfe2fe6ec_i'' \<mapsto> Msg (DoNotUse_68fffe8e525945708a2c302dfe2fe6ec_SenderE x)]"
+"\<lambda>x. [\<C> ''DoNotUse_d60d54060b9d448ea60e06d4478b7275_i'' \<mapsto> Msg (DoNotUse_d60d54060b9d448ea60e06d4478b7275_SenderE x)]"
   unfolding sbElemWell_def
   unfolding usclOkay_stream_def
   unfolding ctype_tsyn_def
   by simp
 
 lift_definition senderElem_raw_ds :: "('e\<times>bool) \<Rightarrow> ('e::countable) senderMessage tsyn sbElem" is
-"\<lambda>x. [\<C> ''DoNotUse_68fffe8e525945708a2c302dfe2fe6ec_ds'' \<mapsto> Msg (DoNotUse_68fffe8e525945708a2c302dfe2fe6ec_SenderPair_E_Bool x)]"
+"\<lambda>x. [\<C> ''DoNotUse_d60d54060b9d448ea60e06d4478b7275_ds'' \<mapsto> Msg (DoNotUse_d60d54060b9d448ea60e06d4478b7275_SenderPair_E_Bool x)]"
   unfolding sbElemWell_def
   unfolding usclOkay_stream_def
   unfolding ctype_tsyn_def
@@ -83,7 +74,7 @@ section \<open>Helpers to create a bundle from a single tsyn element\<close>
 
 fun senderElem_as :: "bool tsyn \<Rightarrow> ('e::countable) senderMessage tsyn sbElem" where
 "senderElem_as (Msg port_as) = senderElem_raw_as port_as" |
-"senderElem_as null = sbeNull {\<C> ''DoNotUse_68fffe8e525945708a2c302dfe2fe6ec_as''}"
+"senderElem_as null = sbeNull {\<C> ''DoNotUse_d60d54060b9d448ea60e06d4478b7275_as''}"
 
 declare senderElem_as.simps[simp del]
 
@@ -92,7 +83,7 @@ definition sender_as :: "bool tsyn \<Rightarrow> ('e::countable) senderMessage t
 
 fun senderElem_i :: "'e tsyn \<Rightarrow> ('e::countable) senderMessage tsyn sbElem" where
 "senderElem_i (Msg port_i) = senderElem_raw_i port_i" |
-"senderElem_i null = sbeNull {\<C> ''DoNotUse_68fffe8e525945708a2c302dfe2fe6ec_i''}"
+"senderElem_i null = sbeNull {\<C> ''DoNotUse_d60d54060b9d448ea60e06d4478b7275_i''}"
 
 declare senderElem_i.simps[simp del]
 
@@ -101,7 +92,7 @@ definition sender_i :: "'e tsyn \<Rightarrow> ('e::countable) senderMessage tsyn
 
 fun senderElem_ds :: "('e\<times>bool) tsyn \<Rightarrow> ('e::countable) senderMessage tsyn sbElem" where
 "senderElem_ds (Msg port_ds) = senderElem_raw_ds port_ds" |
-"senderElem_ds null = sbeNull {\<C> ''DoNotUse_68fffe8e525945708a2c302dfe2fe6ec_ds''}"
+"senderElem_ds null = sbeNull {\<C> ''DoNotUse_d60d54060b9d448ea60e06d4478b7275_ds''}"
 
 declare senderElem_ds.simps[simp del]
 
@@ -129,19 +120,19 @@ section \<open>Helpers to create a bundle from a tsyn list of elements\<close>
 
 fun sender_list_as :: "(bool tsyn) list \<Rightarrow> ('e::countable) senderMessage tsyn SB" where
 "sender_list_as (x#xs) = ubConcEq (sender_as x)\<cdot>(sender_list_as xs)" |
-"sender_list_as []     = ubLeast {\<C> ''DoNotUse_68fffe8e525945708a2c302dfe2fe6ec_as''}"
+"sender_list_as []     = ubLeast {\<C> ''DoNotUse_d60d54060b9d448ea60e06d4478b7275_as''}"
 
 declare sender_list_as.simps[simp del]
 
 fun sender_list_i :: "('e tsyn) list \<Rightarrow> ('e::countable) senderMessage tsyn SB" where
 "sender_list_i (x#xs) = ubConcEq (sender_i x)\<cdot>(sender_list_i xs)" |
-"sender_list_i []     = ubLeast {\<C> ''DoNotUse_68fffe8e525945708a2c302dfe2fe6ec_i''}"
+"sender_list_i []     = ubLeast {\<C> ''DoNotUse_d60d54060b9d448ea60e06d4478b7275_i''}"
 
 declare sender_list_i.simps[simp del]
 
 fun sender_list_ds :: "(('e\<times>bool) tsyn) list \<Rightarrow> ('e::countable) senderMessage tsyn SB" where
 "sender_list_ds (x#xs) = ubConcEq (sender_ds x)\<cdot>(sender_list_ds xs)" |
-"sender_list_ds []     = ubLeast {\<C> ''DoNotUse_68fffe8e525945708a2c302dfe2fe6ec_ds''}"
+"sender_list_ds []     = ubLeast {\<C> ''DoNotUse_d60d54060b9d448ea60e06d4478b7275_ds''}"
 
 declare sender_list_ds.simps[simp del]
 
@@ -158,44 +149,41 @@ fun senderOut_list_ds :: "(('e\<times>bool) tsyn) list \<Rightarrow> ('e::counta
 
 section \<open>Helpers to create a bundle from a tsyn stream of elements\<close>
 
-lift_definition DoNotUse_68fffe8e525945708a2c302dfe2fe6ec_sender_stream_as_h :: "bool tsyn stream \<Rightarrow> ('e::countable) senderMessage tsyn SB" is
-"\<lambda> s. [(\<C> ''DoNotUse_68fffe8e525945708a2c302dfe2fe6ec_as'') \<mapsto> (tsynMap (DoNotUse_68fffe8e525945708a2c302dfe2fe6ec_SenderBool)\<cdot>s)]"
+lift_definition DoNotUse_d60d54060b9d448ea60e06d4478b7275_sender_stream_as_h :: "bool tsyn stream \<Rightarrow> ('e::countable) senderMessage tsyn SB" is
+"\<lambda> s. [(\<C> ''DoNotUse_d60d54060b9d448ea60e06d4478b7275_as'') \<mapsto> (tsynMap (DoNotUse_d60d54060b9d448ea60e06d4478b7275_SenderBool)\<cdot>s)]"
   unfolding ubWell_def usclOkay_stream_def ctype_tsyn_def
-  apply auto (* TODO War angeblich mal fertig, hat jetzt aber noch ein Goal *)
-  sorry
+  by auto
 
 lift_definition sender_stream_as :: "(bool) tsyn stream \<rightarrow> ('e::countable) senderMessage tsyn SB" is
-"DoNotUse_68fffe8e525945708a2c302dfe2fe6ec_sender_stream_as_h"
-  apply(auto simp add: cfun_def DoNotUse_68fffe8e525945708a2c302dfe2fe6ec_sender_stream_as_h_def map_fun_def comp_def)
+"DoNotUse_d60d54060b9d448ea60e06d4478b7275_sender_stream_as_h"
+  apply(auto simp add: cfun_def DoNotUse_d60d54060b9d448ea60e06d4478b7275_sender_stream_as_h_def map_fun_def comp_def)
   apply(rule cont_Abs_UB)
   apply(simp add: option_one_cont)
-  by (metis DoNotUse_68fffe8e525945708a2c302dfe2fe6ec_sender_stream_as_h.rep_eq ubrep_well)
+  by (metis DoNotUse_d60d54060b9d448ea60e06d4478b7275_sender_stream_as_h.rep_eq ubrep_well)
 
-lift_definition DoNotUse_68fffe8e525945708a2c302dfe2fe6ec_sender_stream_i_h :: "'e tsyn stream \<Rightarrow> ('e::countable) senderMessage tsyn SB" is
-"\<lambda> s. [(\<C> ''DoNotUse_68fffe8e525945708a2c302dfe2fe6ec_i'') \<mapsto> (tsynMap (DoNotUse_68fffe8e525945708a2c302dfe2fe6ec_SenderE)\<cdot>s)]"
+lift_definition DoNotUse_d60d54060b9d448ea60e06d4478b7275_sender_stream_i_h :: "'e tsyn stream \<Rightarrow> ('e::countable) senderMessage tsyn SB" is
+"\<lambda> s. [(\<C> ''DoNotUse_d60d54060b9d448ea60e06d4478b7275_i'') \<mapsto> (tsynMap (DoNotUse_d60d54060b9d448ea60e06d4478b7275_SenderE)\<cdot>s)]"
   unfolding ubWell_def usclOkay_stream_def ctype_tsyn_def
-  apply auto (* TODO War angeblich mal fertig, hat jetzt aber noch ein Goal *)
-  sorry
+  by auto
 
 lift_definition sender_stream_i :: "('e) tsyn stream \<rightarrow> ('e::countable) senderMessage tsyn SB" is
-"DoNotUse_68fffe8e525945708a2c302dfe2fe6ec_sender_stream_i_h"
-  apply(auto simp add: cfun_def DoNotUse_68fffe8e525945708a2c302dfe2fe6ec_sender_stream_i_h_def map_fun_def comp_def)
+"DoNotUse_d60d54060b9d448ea60e06d4478b7275_sender_stream_i_h"
+  apply(auto simp add: cfun_def DoNotUse_d60d54060b9d448ea60e06d4478b7275_sender_stream_i_h_def map_fun_def comp_def)
   apply(rule cont_Abs_UB)
   apply(simp add: option_one_cont)
-  by (metis DoNotUse_68fffe8e525945708a2c302dfe2fe6ec_sender_stream_i_h.rep_eq ubrep_well)
+  by (metis DoNotUse_d60d54060b9d448ea60e06d4478b7275_sender_stream_i_h.rep_eq ubrep_well)
 
-lift_definition DoNotUse_68fffe8e525945708a2c302dfe2fe6ec_sender_stream_ds_h :: "('e\<times>bool) tsyn stream \<Rightarrow> ('e::countable) senderMessage tsyn SB" is
-"\<lambda> s. [(\<C> ''DoNotUse_68fffe8e525945708a2c302dfe2fe6ec_ds'') \<mapsto> (tsynMap (DoNotUse_68fffe8e525945708a2c302dfe2fe6ec_SenderPair_E_Bool)\<cdot>s)]"
+lift_definition DoNotUse_d60d54060b9d448ea60e06d4478b7275_sender_stream_ds_h :: "('e\<times>bool) tsyn stream \<Rightarrow> ('e::countable) senderMessage tsyn SB" is
+"\<lambda> s. [(\<C> ''DoNotUse_d60d54060b9d448ea60e06d4478b7275_ds'') \<mapsto> (tsynMap (DoNotUse_d60d54060b9d448ea60e06d4478b7275_SenderPair_E_Bool)\<cdot>s)]"
   unfolding ubWell_def usclOkay_stream_def ctype_tsyn_def
-  apply auto (* TODO War angeblich mal fertig, hat jetzt aber noch ein Goal *)
-  sorry
+  by auto
 
 lift_definition sender_stream_ds :: "(('e\<times>bool)) tsyn stream \<rightarrow> ('e::countable) senderMessage tsyn SB" is
-"DoNotUse_68fffe8e525945708a2c302dfe2fe6ec_sender_stream_ds_h"
-  apply(auto simp add: cfun_def DoNotUse_68fffe8e525945708a2c302dfe2fe6ec_sender_stream_ds_h_def map_fun_def comp_def)
+"DoNotUse_d60d54060b9d448ea60e06d4478b7275_sender_stream_ds_h"
+  apply(auto simp add: cfun_def DoNotUse_d60d54060b9d448ea60e06d4478b7275_sender_stream_ds_h_def map_fun_def comp_def)
   apply(rule cont_Abs_UB)
   apply(simp add: option_one_cont)
-  by (metis DoNotUse_68fffe8e525945708a2c302dfe2fe6ec_sender_stream_ds_h.rep_eq ubrep_well)
+  by (metis DoNotUse_d60d54060b9d448ea60e06d4478b7275_sender_stream_ds_h.rep_eq ubrep_well)
 
 (* Create one SB for all input channels *)
 definition senderIn_stream_as_i :: "bool tsyn stream \<rightarrow> 'e tsyn stream \<rightarrow> ('e::countable) senderMessage tsyn SB" where
@@ -209,24 +197,24 @@ definition senderOut_stream_ds :: "('e\<times>bool) tsyn stream \<rightarrow> ('
 section \<open>Helpers to get tsyn elements and streams from sbElems and SBs\<close>
 
 definition senderElem_get_as :: "('e::countable) senderMessage tsyn sbElem \<Rightarrow> (bool) tsyn" where
-"senderElem_get_as sbe = tsynApplyElem (inv DoNotUse_68fffe8e525945708a2c302dfe2fe6ec_SenderBool) ((Rep_sbElem sbe) \<rightharpoonup> (\<C> ''DoNotUse_68fffe8e525945708a2c302dfe2fe6ec_as''))"
+"senderElem_get_as sbe = tsynApplyElem (inv DoNotUse_d60d54060b9d448ea60e06d4478b7275_SenderBool) ((Rep_sbElem sbe) \<rightharpoonup> (\<C> ''DoNotUse_d60d54060b9d448ea60e06d4478b7275_as''))"
 
 lift_definition sender_get_stream_as :: "('e::countable) senderMessage tsyn SB \<rightarrow> bool tsyn stream" is
-"\<lambda>sb. tsynMap (inv DoNotUse_68fffe8e525945708a2c302dfe2fe6ec_SenderBool)\<cdot>(sb . (\<C> ''DoNotUse_68fffe8e525945708a2c302dfe2fe6ec_as''))"
+"\<lambda>sb. tsynMap (inv DoNotUse_d60d54060b9d448ea60e06d4478b7275_SenderBool)\<cdot>(sb . (\<C> ''DoNotUse_d60d54060b9d448ea60e06d4478b7275_as''))"
   by(simp add: cfun_def)
 
 definition senderElem_get_i :: "('e::countable) senderMessage tsyn sbElem \<Rightarrow> ('e) tsyn" where
-"senderElem_get_i sbe = tsynApplyElem (inv DoNotUse_68fffe8e525945708a2c302dfe2fe6ec_SenderE) ((Rep_sbElem sbe) \<rightharpoonup> (\<C> ''DoNotUse_68fffe8e525945708a2c302dfe2fe6ec_i''))"
+"senderElem_get_i sbe = tsynApplyElem (inv DoNotUse_d60d54060b9d448ea60e06d4478b7275_SenderE) ((Rep_sbElem sbe) \<rightharpoonup> (\<C> ''DoNotUse_d60d54060b9d448ea60e06d4478b7275_i''))"
 
 lift_definition sender_get_stream_i :: "('e::countable) senderMessage tsyn SB \<rightarrow> 'e tsyn stream" is
-"\<lambda>sb. tsynMap (inv DoNotUse_68fffe8e525945708a2c302dfe2fe6ec_SenderE)\<cdot>(sb . (\<C> ''DoNotUse_68fffe8e525945708a2c302dfe2fe6ec_i''))"
+"\<lambda>sb. tsynMap (inv DoNotUse_d60d54060b9d448ea60e06d4478b7275_SenderE)\<cdot>(sb . (\<C> ''DoNotUse_d60d54060b9d448ea60e06d4478b7275_i''))"
   by(simp add: cfun_def)
 
 definition senderElem_get_ds :: "('e::countable) senderMessage tsyn sbElem \<Rightarrow> (('e\<times>bool)) tsyn" where
-"senderElem_get_ds sbe = tsynApplyElem (inv DoNotUse_68fffe8e525945708a2c302dfe2fe6ec_SenderPair_E_Bool) ((Rep_sbElem sbe) \<rightharpoonup> (\<C> ''DoNotUse_68fffe8e525945708a2c302dfe2fe6ec_ds''))"
+"senderElem_get_ds sbe = tsynApplyElem (inv DoNotUse_d60d54060b9d448ea60e06d4478b7275_SenderPair_E_Bool) ((Rep_sbElem sbe) \<rightharpoonup> (\<C> ''DoNotUse_d60d54060b9d448ea60e06d4478b7275_ds''))"
 
 lift_definition sender_get_stream_ds :: "('e::countable) senderMessage tsyn SB \<rightarrow> ('e\<times>bool) tsyn stream" is
-"\<lambda>sb. tsynMap (inv DoNotUse_68fffe8e525945708a2c302dfe2fe6ec_SenderPair_E_Bool)\<cdot>(sb . (\<C> ''DoNotUse_68fffe8e525945708a2c302dfe2fe6ec_ds''))"
+"\<lambda>sb. tsynMap (inv DoNotUse_d60d54060b9d448ea60e06d4478b7275_SenderPair_E_Bool)\<cdot>(sb . (\<C> ''DoNotUse_d60d54060b9d448ea60e06d4478b7275_ds''))"
   by(simp add: cfun_def)
 
 
@@ -358,17 +346,17 @@ lemma senderautomaton_ran[simp]: "daRan senderAutomaton = senderRan"
 
 section \<open>Lemmas for single tsyn setter\<close>
 
-lemma senderelem_as_dom[simp]: "sbeDom (senderElem_as x) = {\<C> ''DoNotUse_68fffe8e525945708a2c302dfe2fe6ec_as''}"
+lemma senderelem_as_dom[simp]: "sbeDom (senderElem_as x) = {\<C> ''DoNotUse_d60d54060b9d448ea60e06d4478b7275_as''}"
   apply(cases x)
   apply(simp add: senderElem_as.simps sbeDom_def senderElem_raw_as.rep_eq)
   by(simp add: senderElem_as.simps)
 
-lemma senderelem_i_dom[simp]: "sbeDom (senderElem_i x) = {\<C> ''DoNotUse_68fffe8e525945708a2c302dfe2fe6ec_i''}"
+lemma senderelem_i_dom[simp]: "sbeDom (senderElem_i x) = {\<C> ''DoNotUse_d60d54060b9d448ea60e06d4478b7275_i''}"
   apply(cases x)
   apply(simp add: senderElem_i.simps sbeDom_def senderElem_raw_i.rep_eq)
   by(simp add: senderElem_i.simps)
 
-lemma senderelem_ds_dom[simp]: "sbeDom (senderElem_ds x) = {\<C> ''DoNotUse_68fffe8e525945708a2c302dfe2fe6ec_ds''}"
+lemma senderelem_ds_dom[simp]: "sbeDom (senderElem_ds x) = {\<C> ''DoNotUse_d60d54060b9d448ea60e06d4478b7275_ds''}"
   apply(cases x)
   apply(simp add: senderElem_ds.simps sbeDom_def senderElem_raw_ds.rep_eq)
   by(simp add: senderElem_ds.simps)
@@ -430,16 +418,19 @@ lemma sender_stream_ds_id[simp]: "sender_get_stream_ds\<cdot>(sender_stream_ds\<
 subsection \<open>Identity lemmas for input sbElems\<close>
 
 lemma senderelemin_as_i_as_id[simp]: "senderElem_get_as (senderElemIn_as_i port_as port_i) = port_as"
-  sorry
+  apply(simp add: senderElemIn_as_i_def senderElem_get_as_def)
+  by(metis senderElem_get_as_def senderelem_as_id)
 
 lemma senderelemin_as_i_i_id[simp]: "senderElem_get_i (senderElemIn_as_i port_as port_i) = port_i"
-  sorry
+  apply(simp add: senderElemIn_as_i_def senderElem_get_i_def)
+  by(metis senderElem_get_i_def senderelem_i_id)
 
 
 subsection \<open>Identity lemmas for output sbElems\<close>
 
 lemma senderelemout_ds_ds_id[simp]: "senderElem_get_ds (senderElemOut_ds port_ds) = port_ds"
-  sorry
+  apply(simp add: senderElemOut_ds_def senderElem_get_ds_def)
+  by(metis senderElem_get_ds_def senderelem_ds_id)
 
 
 subsection \<open>Identity lemmas for input SBs\<close>
@@ -451,9 +442,9 @@ lemma senderin_as_i_as_id[simp]: "sender_get_stream_as\<cdot>(senderIn_as_i port
   apply(cases port_as)
   apply(auto simp add: senderElem_as.simps)
   unfolding senderElem_get_as_def senderElem_raw_as.rep_eq
-  (* TODO Ab hier funktioniert der Beweis nicht mehr *)
-  (*apply auto
-  apply (meson f_inv_into_f rangeI senderMessage.inject(1))
+  apply auto
+  (* TODO not working for SenderAutomaton *)
+  (*apply (meson f_inv_into_f rangeI senderMessage.inject(1))
   by(simp add: sbeNull.rep_eq)*)
   sorry
 
@@ -464,9 +455,9 @@ lemma senderin_as_i_i_id[simp]: "sender_get_stream_i\<cdot>(senderIn_as_i port_a
   apply(cases port_i)
   apply(auto simp add: senderElem_i.simps)
   unfolding senderElem_get_i_def senderElem_raw_i.rep_eq
-  (* TODO Ab hier funktioniert der Beweis nicht mehr *)
-  (*apply auto
-  apply (meson f_inv_into_f rangeI senderMessage.inject(1))
+  apply auto
+  (* TODO not working for SenderAutomaton *)
+  (*apply (meson f_inv_into_f rangeI senderMessage.inject(1))
   by(simp add: sbeNull.rep_eq)*)
   sorry
 
@@ -474,6 +465,16 @@ lemma senderin_as_i_i_id[simp]: "sender_get_stream_i\<cdot>(senderIn_as_i port_a
 subsection \<open>Identity lemmas for output SBs\<close>
 
 lemma senderout_ds_ds_id[simp]: "sender_get_stream_ds\<cdot>(senderOut_ds port_ds) = \<up>port_ds"
+  apply(simp add: sender_get_stream_ds_def senderOut_ds_def)
+  apply(subst sbe2sb_getch)
+  apply(auto simp add: senderDom_def senderElemOut_ds_def)
+  apply(cases port_ds)
+  apply(auto simp add: senderElem_ds.simps)
+  unfolding senderElem_get_ds_def senderElem_raw_ds.rep_eq
+  apply auto
+  (* TODO not working for SenderAutomaton *)
+  (*apply (meson f_inv_into_f rangeI senderMessage.inject(1))
+  by(simp add: sbeNull.rep_eq)*)
   sorry
 
 
